tuned names and optimized comparison order

src/HOL/Data_Structures/AList_Upd_Del.thy
@@ -14,39 +14,39 @@ amount of lemmas implicitly (via the simpset). *}
 hide_const (open) map_of
 
 fun map_of :: "('a*'b)list \<Rightarrow> 'a \<Rightarrow> 'b option" where
-"map_of [] = (\<lambda>a. None)" |
-"map_of ((x,y)#ps) = (\<lambda>a. if x=a then Some y else map_of ps a)"
+"map_of [] = (\<lambda>x. None)" |
+"map_of ((a,b)#ps) = (\<lambda>x. if x=a then Some b else map_of ps x)"
 
 text \<open>Updating an association list:\<close>
 
 fun upd_list :: "'a::linorder \<Rightarrow> 'b \<Rightarrow> ('a*'b) list \<Rightarrow> ('a*'b) list" where
-"upd_list a b [] = [(a,b)]" |
-"upd_list a b ((x,y)#ps) =
-  (if a < x then (a,b)#(x,y)#ps else
-  if a=x then (a,b)#ps else (x,y) # upd_list a b ps)"
+"upd_list x y [] = [(x,y)]" |
+"upd_list x y ((a,b)#ps) =
+  (if x < a then (x,y)#(a,b)#ps else
+  if x = a then (x,y)#ps else (a,b) # upd_list x y ps)"
 
 fun del_list :: "'a::linorder \<Rightarrow> ('a*'b)list \<Rightarrow> ('a*'b)list" where
-"del_list a [] = []" |
-"del_list a ((x,y)#ps) = (if a=x then ps else (x,y) # del_list a ps)"
+"del_list x [] = []" |
+"del_list x ((a,b)#ps) = (if x = a then ps else (a,b) # del_list x ps)"
 
 
 subsection \<open>Lemmas for @{const map_of}\<close>
 
-lemma map_of_ins_list: "map_of (upd_list a b ps) = (map_of ps)(a := Some b)"
+lemma map_of_ins_list: "map_of (upd_list x y ps) = (map_of ps)(x := Some y)"
 by(induction ps) auto
 
-lemma map_of_append: "map_of (ps @ qs) a =
-  (case map_of ps a of None \<Rightarrow> map_of qs a | Some b \<Rightarrow> Some b)"
+lemma map_of_append: "map_of (ps @ qs) x =
+  (case map_of ps x of None \<Rightarrow> map_of qs x | Some y \<Rightarrow> Some y)"
 by(induction ps)(auto)
 
-lemma map_of_None: "sorted (a # map fst ps) \<Longrightarrow> map_of ps a = None"
+lemma map_of_None: "sorted (x # map fst ps) \<Longrightarrow> map_of ps x = None"
 by (induction ps) (auto simp: sorted_lems sorted_Cons_iff)
 
-lemma map_of_None2: "sorted (map fst ps @ [a]) \<Longrightarrow> map_of ps a = None"
+lemma map_of_None2: "sorted (map fst ps @ [x]) \<Longrightarrow> map_of ps x = None"
 by (induction ps) (auto simp: sorted_lems)
 
 lemma map_of_del_list: "sorted1 ps \<Longrightarrow>
-  map_of(del_list a ps) = (map_of ps)(a := None)"
+  map_of(del_list x ps) = (map_of ps)(x := None)"
 by(induction ps) (auto simp: map_of_None sorted_lems fun_eq_iff)
 
 lemma map_of_sorted_Cons: "sorted (a # map fst ps) \<Longrightarrow> x < a \<Longrightarrow>
@@ -63,19 +63,19 @@ lemmas map_of_simps = sorted_lems map_of_append map_of_sorteds
 
 subsection \<open>Lemmas for @{const upd_list}\<close>
 
-lemma sorted_upd_list: "sorted1 ps \<Longrightarrow> sorted1 (upd_list a b ps)"
-apply(induction ps) 
+lemma sorted_upd_list: "sorted1 ps \<Longrightarrow> sorted1 (upd_list x y ps)"
+apply(induction ps)
  apply simp
 apply(case_tac ps)
  apply auto
 done
 
-lemma upd_list_sorted1: "\<lbrakk> sorted (map fst ps @ [x]); a < x \<rbrakk> \<Longrightarrow>
-  upd_list a b (ps @ (x,y) # qs) =  upd_list a b ps @ (x,y) # qs"
+lemma upd_list_sorted1: "\<lbrakk> sorted (map fst ps @ [a]); x < a \<rbrakk> \<Longrightarrow>
+  upd_list x y (ps @ (a,b) # qs) =  upd_list x y ps @ (a,b) # qs"
 by(induction ps) (auto simp: sorted_lems)
 
-lemma upd_list_sorted2: "\<lbrakk> sorted (map fst ps @ [x]); x \<le> a \<rbrakk> \<Longrightarrow>
-  upd_list a b (ps @ (x,y) # qs) = ps @ upd_list a b ((x,y)#qs)"
+lemma upd_list_sorted2: "\<lbrakk> sorted (map fst ps @ [a]); a \<le> x \<rbrakk> \<Longrightarrow>
+  upd_list x y (ps @ (a,b) # qs) = ps @ upd_list x y ((a,b) # qs)"
 by(induction ps) (auto simp: sorted_lems)
 
 lemmas upd_list_simps = sorted_lems upd_list_sorted1 upd_list_sorted2
@@ -110,28 +110,28 @@ by (meson order.strict_trans sorted_Cons_iff)
 lemma del_list_idem: "x \<notin> set(map fst xs) \<Longrightarrow> del_list x xs = xs"
 by (induct xs) auto
 
-lemma del_list_sorted1: "sorted1 (xs @ [(x,y)]) \<Longrightarrow> x \<le> a \<Longrightarrow>
-  del_list a (xs @ (x,y) # ys) = xs @ del_list a ((x,y) # ys)"
+lemma del_list_sorted1: "sorted1 (xs @ [(a,b)]) \<Longrightarrow> a \<le> x \<Longrightarrow>
+  del_list x (xs @ (a,b) # ys) = xs @ del_list x ((a,b) # ys)"
 by (induction xs) (auto simp: sorted_mid_iff2)
 
-lemma del_list_sorted2: "sorted1 (xs @ (x,y) # ys) \<Longrightarrow> a < x \<Longrightarrow>
-  del_list a (xs @ (x,y) # ys) = del_list a xs @ (x,y) # ys"
+lemma del_list_sorted2: "sorted1 (xs @ (a,b) # ys) \<Longrightarrow> x < a \<Longrightarrow>
+  del_list x (xs @ (a,b) # ys) = del_list x xs @ (a,b) # ys"
 by (induction xs) (fastforce simp: sorted_Cons_iff intro!: del_list_idem)+
 
 lemma del_list_sorted3:
-  "sorted1 (xs @ (x,x') # ys @ (y,y') # zs) \<Longrightarrow> a < y \<Longrightarrow>
-  del_list a (xs @ (x,x') # ys @ (y,y') # zs) = del_list a (xs @ (x,x') # ys) @ (y,y') # zs"
+  "sorted1 (xs @ (a,a') # ys @ (b,b') # zs) \<Longrightarrow> x < b \<Longrightarrow>
+  del_list x (xs @ (a,a') # ys @ (b,b') # zs) = del_list x (xs @ (a,a') # ys) @ (b,b') # zs"
 by (induction xs) (auto simp: sorted_Cons_iff del_list_sorted2 ball_Un)
 
 lemma del_list_sorted4:
-  "sorted1 (xs @ (x,x') # ys @ (y,y') # zs @ (z,z') # us) \<Longrightarrow> a < z \<Longrightarrow>
-  del_list a (xs @ (x,x') # ys @ (y,y') # zs @ (z,z') # us) = del_list a (xs @ (x,x') # ys @ (y,y') # zs) @ (z,z') # us"
+  "sorted1 (xs @ (a,a') # ys @ (b,b') # zs @ (c,c') # us) \<Longrightarrow> x < c \<Longrightarrow>
+  del_list x (xs @ (a,a') # ys @ (b,b') # zs @ (c,c') # us) = del_list x (xs @ (a,a') # ys @ (b,b') # zs) @ (c,c') # us"
 by (induction xs) (auto simp: sorted_Cons_iff del_list_sorted3)
 
 lemma del_list_sorted5:
-  "sorted1 (xs @ (x,x') # ys @ (y,y') # zs @ (z,z') # us @ (u,u') # vs) \<Longrightarrow> a < u \<Longrightarrow>
-   del_list a (xs @ (x,x') # ys @ (y,y') # zs @ (z,z') # us @ (u,u') # vs) =
-   del_list a (xs @ (x,x') # ys @ (y,y') # zs @ (z,z') # us) @ (u,u') # vs" 
+  "sorted1 (xs @ (a,a') # ys @ (b,b') # zs @ (c,c') # us @ (d,d') # vs) \<Longrightarrow> x < d \<Longrightarrow>
+   del_list x (xs @ (a,a') # ys @ (b,b') # zs @ (c,c') # us @ (d,d') # vs) =
+   del_list x (xs @ (a,a') # ys @ (b,b') # zs @ (c,c') # us) @ (d,d') # vs" 
 by (induction xs) (auto simp: sorted_Cons_iff del_list_sorted4)
 
 lemmas del_list_sorted =
